in the middle of refactoring. current state: all is broken

thy/Primitive_Matchers/IpAddresses.thy
@@ -40,14 +40,14 @@ by(simp add: ipv4addr_of_dotdecimal.simps ipv4addr_of_nat_def ipv4range_set_from
 
   (*TODO: remove this lemma?, refactor*)
   lemma ipv4cidr_to_interval: "ipcidr_to_interval (base, len) = (s,e) \<Longrightarrow> ipv4range_set_from_prefix base len = {s .. e}"
+    apply(subst transition_lemma_ipv4_delete_me)
     apply(simp add: Let_def ipcidr_to_interval_def)
-    thm ipset_from_cidr_ipcidr_to_interval
-    using ipset_from_cidr_ipcidr_to_interval by presburger
+    using ipset_from_cidr_ipcidr_to_interval by blast
 
 
 
-  fun ipv4cidr_conjunct :: "('i::len word \<times> nat) \<Rightarrow> ('i word \<times> nat) \<Rightarrow> ('i word \<times> nat) option" where 
-    "ipv4cidr_conjunct (base1, m1) (base2, m2) = (if ipset_from_cidr base1 m1 \<inter> ipset_from_cidr base2 m2 = {}
+  fun ipcidr_conjunct :: "('i::len word \<times> nat) \<Rightarrow> ('i word \<times> nat) \<Rightarrow> ('i word \<times> nat) option" where 
+    "ipcidr_conjunct (base1, m1) (base2, m2) = (if ipset_from_cidr base1 m1 \<inter> ipset_from_cidr base2 m2 = {}
        then
         None
        else if 
@@ -58,11 +58,14 @@ by(simp add: ipv4addr_of_dotdecimal.simps ipv4addr_of_nat_def ipv4range_set_from
         Some (base2, m2)
       )"
   
-  lemma ipv4cidr_conjunct_correct: "(case ipv4cidr_conjunct (b1, m1) (b2, m2) of Some (bx, mx) \<Rightarrow> ipv4range_set_from_prefix bx mx | None \<Rightarrow> {}) = 
-      (ipv4range_set_from_prefix b1 m1) \<inter> (ipv4range_set_from_prefix b2 m2)"
+  lemma ipcidr_conjunct_correct: "(case ipcidr_conjunct (b1, m1) (b2, m2)
+                                          of Some (bx, mx) \<Rightarrow> ipset_from_cidr bx mx
+                                          |  None \<Rightarrow> {})
+      = 
+      (ipset_from_cidr b1 m1) \<inter> (ipset_from_cidr b2 m2)"
     apply(simp split: split_if_asm)
     using ip_cidr_intersect by fast
-  declare ipv4cidr_conjunct.simps[simp del]
+  declare ipcidr_conjunct.simps[simp del]
 
   (*TODO: this is a duplicate, right?*)
   definition ipv4_cidr_tuple_to_interval :: "(ipv4addr \<times> nat) \<Rightarrow> 32 wordinterval" where
@@ -70,11 +73,12 @@ by(simp add: ipv4addr_of_dotdecimal.simps ipv4addr_of_nat_def ipv4range_set_from
 
   lemma wordinterval_to_set_ipv4_cidr_tuple_to_interval:
     "wordinterval_to_set (ipv4_cidr_tuple_to_interval (b, m)) = ipv4range_set_from_prefix b m"
+    apply(subst transition_lemma_ipv4_delete_me)
     unfolding ipv4_cidr_tuple_to_interval_def ipset_from_cidr_ipcidr_to_interval ipcidr_to_interval_def
     by(simp add: ipv4range_range.simps ipv4range_to_set_def)
 
   lemma [code_unfold]: 
-  "ipv4cidr_conjunct ips1 ips2 = (if wordinterval_empty (wordinterval_intersection (ipv4_cidr_tuple_to_interval ips1) (ipv4_cidr_tuple_to_interval ips2))
+  "ipcidr_conjunct ips1 ips2 = (if wordinterval_empty (wordinterval_intersection (ipv4_cidr_tuple_to_interval ips1) (ipv4_cidr_tuple_to_interval ips2))
        then
         None
        else if 
@@ -87,9 +91,9 @@ by(simp add: ipv4addr_of_dotdecimal.simps ipv4addr_of_nat_def ipv4range_set_from
   apply(simp)
   apply(cases ips1, cases ips2, rename_tac b1 m1 b2 m2, simp)
   apply(safe)
-     apply(auto simp add: wordinterval_to_set_ipv4_cidr_tuple_to_interval ipv4cidr_conjunct.simps split:split_if_asm)
+     apply(auto simp add: wordinterval_to_set_ipv4_cidr_tuple_to_interval ipcidr_conjunct.simps split:split_if_asm)
   done
-  value "ipv4cidr_conjunct (0,0) (8,1)" (*with the code_unfold lemma before, this works!*)
+  value "ipcidr_conjunct (0,0) (8,1)" (*with the code_unfold lemma before, this works!*)
 
   
   (*TODO: generalize, move*)
@@ -112,6 +116,7 @@ by(simp add: ipv4addr_of_dotdecimal.simps ipv4addr_of_nat_def ipv4range_set_from
     apply(simp add: ipcidr_to_interval_def)
     apply(simp add: ipset_from_cidr_ipcidr_to_interval)
     done
+    sorry
   
 
 
